Flapjack/Test/Allocator.lean
@@ -111,4 +111,43 @@ example [OfNat α 1] :
     wordApplyColour, wordApplyColourExp, wordMapVars, lookupNatInfo,
     List.eraseDups, List.eraseDupsBy, List.eraseDupsBy.loop]
 
+example :
+    wordSsaRenameProgram
+        ({ current := [(2, 100)], next := 200 } : WordSsaState)
+        ((.shareInst .load 1
+          (.op .add [.var 2, .const (4 : Nat)])) : WordProg Nat) =
+        ({ current := [(1, 200), (2, 100)], next := 201 },
+        .shareInst .load 200 (.op .add [.var 100, .const 4])) := by
+  simp [wordSsaRenameProgram, wordSsaRenameExp, wordSsaFresh,
+    wordSsaRead, lookupNatInfo]
+
+example :
+    wordSsaRenameProgram
+        ({ current := [(2, 100)], next := 200 } : WordSsaState)
+        ((.call (some ([3, 4], [2])) (some 7) [2, 5] none) : WordProg Nat) =
+        ({ current := [(4, 201), (3, 200), (2, 100)], next := 202 },
+        .call (some ([200, 201], [100])) (some 7) [100, 5] none) := by
+  simp [wordSsaRenameProgram, wordSsaRenameReturns, wordSsaFreshList,
+    wordSsaFresh, wordSsaRead, lookupNatInfo]
+
+example :
+    wordSsaRenameProgram
+        ({ current := [(2, 100)], next := 200 } : WordSsaState)
+        ((.seq (.locValue 3 2) (.return 0 [3])) : WordProg Nat) =
+      ({ current := [(3, 200), (2, 100)], next := 201 },
+        .seq (.locValue 200 100) (.return 0 [200])) := by
+  rfl
+
+example :
+    wordProgReadVars
+        ((.call (some ([5], [6])) (some 7) [8]
+          (some (9, .return 0 [10])) : WordProg Nat)) = [8, 6, 10] := by
+  rfl
+
+example :
+    wordProgWriteVars
+        ((.call (some ([5], [6])) (some 7) [8]
+          (some (9, .return 0 [10])) : WordProg Nat)) = [5, 9] := by
+  rfl
+
 end Flapjack
